Re-organize the invariants of the IL2 proof

compiler/proofs/toIntLang2ProofScript.sml
@@ -90,164 +90,149 @@ val funs_to_i2_map = Q.prove (
  PairCases_on `h` >>
  rw [exp_to_i2_def]);
 
-val lookup_type_tag_def = Define `
-(lookup_type_tag NONE cenv = SOME tuple_tag) ∧
-(lookup_type_tag (SOME cn) (next,env,type_cenv,inv) = FLOOKUP type_cenv cn)`;
-
 val has_exns_def = Define `
-has_exns (cenv, clengths) ⇔
-  FLOOKUP clengths ("Bind", TypeExn NONE) = SOME (0:num) ∧
-  FLOOKUP clengths ("Div", TypeExn NONE) = SOME 0 ∧
-  FLOOKUP clengths ("Eq", TypeExn NONE) = SOME 0 ∧
-  FLOOKUP cenv ("Bind", TypeExn NONE) = SOME bind_tag ∧
-  FLOOKUP cenv ("Div", TypeExn NONE) = SOME div_tag ∧
-  FLOOKUP cenv ("Eq", TypeExn NONE) = SOME eq_tag`;
+has_exns gtagenv ⇔
+  FLOOKUP gtagenv ("Bind", TypeExn NONE) = SOME (bind_tag,0:num) ∧
+  FLOOKUP gtagenv ("Div", TypeExn NONE) = SOME (div_tag,0) ∧
+  FLOOKUP gtagenv ("Eq", TypeExn NONE) = SOME (eq_tag,0)`;
 
 val cenv_inv_def = Define `
-cenv_inv (cenv:envC) ((next, lex_cenv, type_cenv, inverse_cenv):cenv_mapping) (clengths:(conN#tid_or_exn)|-> num) ⇔
+cenv_inv envC tagenv gtagenv ⇔
   (!cn num_args t.
-    lookup_con_id cn cenv = SOME (num_args, t)
+    lookup_con_id cn envC = SOME (num_args, t)
     ⇒
-    FLOOKUP clengths (id_to_n cn,t) = SOME num_args ∧
     ?tag.
-      FLOOKUP lex_cenv cn = SOME tag ∧
-      FLOOKUP type_cenv (id_to_n cn, t) = SOME tag) ∧
-  (!cn. FLOOKUP type_cenv cn ≠ SOME tuple_tag) ∧
-  has_exns (type_cenv,clengths) ∧
-  (!t1 t2 tag cn cn'.
+      lookup_tag_env (SOME cn) tagenv = tag ∧
+      FLOOKUP gtagenv (id_to_n cn, t) = SOME (tag,num_args)) ∧
+  (!cn l. FLOOKUP gtagenv cn ≠ SOME (tuple_tag,l)) ∧
+  has_exns gtagenv ∧
+  (!t1 t2 tag l1 l2 cn cn'.
      (* Comment out same_tid because we're not using separate tag spaces per type *)
      (* same_tid t1 t2 ∧ *)
-     FLOOKUP type_cenv (cn,t1) = SOME tag ∧
-     FLOOKUP type_cenv (cn',t2) = SOME tag
+     FLOOKUP gtagenv (cn,t1) = SOME (tag,l1) ∧
+     FLOOKUP gtagenv (cn',t2) = SOME (tag,l2)
      ⇒
      cn = cn' ∧ t1 = t2)`;
 
 val (v_to_i2_rules, v_to_i2_ind, v_to_i2_cases) = Hol_reln `
-(!cenv lit.
-  v_to_i2 cenv (Litv_i1 lit) (Litv_i2 lit)) ∧
-(!cenv vs vs'.
-  vs_to_i2 cenv vs vs'
+(!gtagenv lit.
+  v_to_i2 gtagenv (Litv_i1 lit) (Litv_i2 lit)) ∧
+(!gtagenv vs vs'.
+  vs_to_i2 gtagenv vs vs'
   ⇒ 
-  v_to_i2 cenv (Conv_i1 NONE vs) (Conv_i2 tuple_tag vs')) ∧
-(!cenv clengths cn tn tag vs vs'.
-  FLOOKUP cenv (cn,tn) = SOME tag ∧
-  FLOOKUP clengths (cn,tn) = SOME (LENGTH vs) ∧
-  vs_to_i2 (cenv,clengths) vs vs'
+  v_to_i2 gtagenv (Conv_i1 NONE vs) (Conv_i2 tuple_tag vs')) ∧
+(!gtagenv cn tn tag vs vs'.
+  FLOOKUP gtagenv (cn,tn) = SOME (tag, LENGTH vs) ∧
+  vs_to_i2 gtagenv vs vs'
   ⇒ 
-  v_to_i2 (cenv,clengths) (Conv_i1 (SOME (cn,tn)) vs) (Conv_i2 tag vs')) ∧
-(!cenv env x e env_i2 envC next lex_cenv inverse_cenv.
-  env_to_i2 (cenv,clengths) env env_i2 ∧
-  cenv_inv envC (next, lex_cenv, cenv, inverse_cenv) clengths
+  v_to_i2 gtagenv (Conv_i1 (SOME (cn,tn)) vs) (Conv_i2 tag vs')) ∧
+(!gtagenv env x e env_i2 envC tagenv.
+  env_to_i2 gtagenv env env_i2 ∧
+  cenv_inv envC tagenv gtagenv
   ⇒ 
-  v_to_i2 (cenv,clengths) (Closure_i1 (envC,env) x e) (Closure_i2 env_i2 x (exp_to_i2 lex_cenv e))) ∧ 
-(!cenv env funs x envC env_i2 next lex_cenv inverse_cenv.
-  env_to_i2 (cenv,clengths) env env_i2 ∧
-  cenv_inv envC (next, lex_cenv, cenv, inverse_cenv) clengths
+  v_to_i2 gtagenv (Closure_i1 (envC,env) x e) (Closure_i2 env_i2 x (exp_to_i2 tagenv e))) ∧ 
+(!gtagenv env funs x envC env_i2 tagenv.
+  env_to_i2 gtagenv env env_i2 ∧
+  cenv_inv envC tagenv gtagenv
   ⇒ 
-  v_to_i2 (cenv,clengths) (Recclosure_i1 (envC,env) funs x) (Recclosure_i2 env_i2 (funs_to_i2 lex_cenv funs) x)) ∧
-(!cenv loc.
-  v_to_i2 cenv (Loc_i1 loc) (Loc_i2 loc)) ∧
-(!cenv.
-  vs_to_i2 cenv [] []) ∧
-(!cenv v vs v' vs'.
-  v_to_i2 cenv v v' ∧
-  vs_to_i2 cenv vs vs'
+  v_to_i2 gtagenv (Recclosure_i1 (envC,env) funs x) (Recclosure_i2 env_i2 (funs_to_i2 tagenv funs) x)) ∧
+(!gtagenv loc.
+  v_to_i2 gtagenv (Loc_i1 loc) (Loc_i2 loc)) ∧
+(!gtagenv.
+  vs_to_i2 gtagenv [] []) ∧
+(!gtagenv v vs v' vs'.
+  v_to_i2 gtagenv v v' ∧
+  vs_to_i2 gtagenv vs vs'
   ⇒
-  vs_to_i2 cenv (v::vs) (v'::vs')) ∧
-(!cenv.
-  env_to_i2 cenv [] []) ∧
-(!cenv x v env env' v'. 
-  env_to_i2 cenv env env' ∧
-  v_to_i2 cenv v v'
+  vs_to_i2 gtagenv (v::vs) (v'::vs')) ∧
+(!gtagenv.
+  env_to_i2 gtagenv [] []) ∧
+(!gtagenv x v env env' v'. 
+  env_to_i2 gtagenv env env' ∧
+  v_to_i2 gtagenv v v'
   ⇒ 
-  env_to_i2 cenv ((x,v)::env) ((x,v')::env'))`;
+  env_to_i2 gtagenv ((x,v)::env) ((x,v')::env'))`;
 
 val v_to_i2_eqns = Q.prove (
-`(!cenv l v.
-  v_to_i2 cenv (Litv_i1 l) v ⇔ 
+`(!gtagenv l v.
+  v_to_i2 gtagenv (Litv_i1 l) v ⇔ 
     (v = Litv_i2 l)) ∧
- (!cenv cn vs v.
-  v_to_i2 cenv (Conv_i1 cn vs) v ⇔ 
-    (?vs' tag cenv' clengths.
-       vs_to_i2 cenv vs vs' ∧ (v = Conv_i2 tag vs') ∧
+ (!gtagenv cn vs v.
+  v_to_i2 gtagenv (Conv_i1 cn vs) v ⇔ 
+    (?vs' tag gtagenv' clengths.
+       vs_to_i2 gtagenv vs vs' ∧ (v = Conv_i2 tag vs') ∧
        (cn = NONE ∧ tag = tuple_tag ∨
-        ?cenv' clengths cn' tn.
-          cenv = (cenv',clengths) ∧
-          FLOOKUP cenv' (cn',tn) = SOME tag ∧
-          FLOOKUP clengths (cn',tn) = SOME (LENGTH vs) ∧
-          cn = SOME (cn',tn) ∧ FLOOKUP cenv' (cn', tn) = SOME tag))) ∧
- (!cenv l v.
-  v_to_i2 cenv (Loc_i1 l) v ⇔ 
+        ?cn' tn.
+          FLOOKUP gtagenv (cn',tn) = SOME (tag,LENGTH vs) ∧
+          cn = SOME (cn',tn)))) ∧
+ (!gtagenv l v.
+  v_to_i2 gtagenv (Loc_i1 l) v ⇔ 
     (v = Loc_i2 l)) ∧
- (!cenv vs.
-  vs_to_i2 cenv [] vs ⇔ 
+ (!gtagenv vs.
+  vs_to_i2 gtagenv [] vs ⇔ 
     (vs = [])) ∧
- (!cenv l v vs vs'.
-  vs_to_i2 cenv (v::vs) vs' ⇔ 
-    ?v' vs''. v_to_i2 cenv v v' ∧ vs_to_i2 cenv vs vs'' ∧ vs' = v'::vs'') ∧
- (!cenv env'.
-  env_to_i2 cenv [] env' ⇔
+ (!gtagenv l v vs vs'.
+  vs_to_i2 gtagenv (v::vs) vs' ⇔ 
+    ?v' vs''. v_to_i2 gtagenv v v' ∧ vs_to_i2 gtagenv vs vs'' ∧ vs' = v'::vs'') ∧
+ (!gtagenv env'.
+  env_to_i2 gtagenv [] env' ⇔
     env' = []) ∧
- (!cenv x v env env'.
-  env_to_i2 cenv ((x,v)::env) env' ⇔
-    ?v' env''. v_to_i2 cenv v v' ∧ env_to_i2 cenv env env'' ∧ env' = ((x,v')::env''))`,
+ (!gtagenv x v env env'.
+  env_to_i2 gtagenv ((x,v)::env) env' ⇔
+    ?v' env''. v_to_i2 gtagenv v v' ∧ env_to_i2 gtagenv env env'' ∧ env' = ((x,v')::env''))`,
 rw [] >>
 rw [Once v_to_i2_cases] >>
 metis_tac []);
 
-val cenv_weak_def = Define `
-cenv_weak (cenv1,clengths1) (cenv2,clengths2) ⇔
-  cenv1 SUBMAP cenv2 ∧
-  clengths1 SUBMAP clengths2 ∧
-  (!cn. FLOOKUP cenv2 cn ≠ SOME tuple_tag) ∧
-  (!t1 t2 tag cn cn'.
+val gtagenv_weak_def = Define `
+gtagenv_weak gtagenv1 gtagenv2 ⇔
+  gtagenv1 SUBMAP gtagenv2 ∧
+  (!cn l. FLOOKUP gtagenv2 cn ≠ SOME (tuple_tag,l)) ∧
+  (!t1 t2 tag cn cn' l1 l2.
      (* Comment out same_tid because we're not using separate tag spaces per type *)
      (* same_tid t1 t2 ∧ *)
-     FLOOKUP cenv2 (cn,t1) = SOME tag ∧
-     FLOOKUP cenv2 (cn',t2) = SOME tag
+     FLOOKUP gtagenv2 (cn,t1) = SOME (tag,l1) ∧
+     FLOOKUP gtagenv2 (cn',t2) = SOME (tag,l2)
      ⇒
      cn = cn' ∧ t1 = t2)`;
 
 val v_to_i2_weakening = Q.prove (
-`(!cenv v v_i2.
-  v_to_i2 cenv v v_i2
+`(!gtagenv v v_i2.
+  v_to_i2 gtagenv v v_i2
   ⇒
-    !cenv'. cenv_weak cenv cenv'
+    !gtagenv'. gtagenv_weak gtagenv gtagenv'
     ⇒
-    v_to_i2 cenv' v v_i2) ∧
- (!cenv vs vs_i2.
-  vs_to_i2 cenv vs vs_i2
+    v_to_i2 gtagenv' v v_i2) ∧
+ (!gtagenv vs vs_i2.
+  vs_to_i2 gtagenv vs vs_i2
   ⇒
-   !cenv'. cenv_weak cenv cenv'
+   !gtagenv'. gtagenv_weak gtagenv gtagenv'
     ⇒
-    vs_to_i2 cenv' vs vs_i2) ∧
- (!cenv env env_i2.
-  env_to_i2 cenv env env_i2
+    vs_to_i2 gtagenv' vs vs_i2) ∧
+ (!gtagenv env env_i2.
+  env_to_i2 gtagenv env env_i2
   ⇒
-   !cenv'. cenv_weak cenv cenv'
+   !gtagenv'. gtagenv_weak gtagenv gtagenv'
     ⇒
-    env_to_i2 cenv' env env_i2)`,
+    env_to_i2 gtagenv' env env_i2)`,
  ho_match_mp_tac v_to_i2_ind >>
- rw [v_to_i2_eqns, cenv_weak_def] >>
+ rw [v_to_i2_eqns, gtagenv_weak_def] >>
  res_tac >>
- `?cenv1 clengths1. cenv' = (cenv1,clengths1)` by metis_tac [pair_CASES] >>
- fs [cenv_weak_def]
+ fs [gtagenv_weak_def]
  >- metis_tac [FLOOKUP_SUBMAP]
  >- (rw [Once v_to_i2_cases] >>
-     Q.LIST_EXISTS_TAC [`next`, `lex_cenv`, `inverse_cenv`] >> 
+     qexists_tac `tagenv` >>
      fs [cenv_inv_def] >>
      rw []
-     >- metis_tac [FLOOKUP_SUBMAP]
      >- metis_tac [FLOOKUP_SUBMAP]
      >- (fs [has_exns_def] >>
          metis_tac [FLOOKUP_SUBMAP])
      >- metis_tac []
      >- metis_tac [])
  >- (rw [Once v_to_i2_cases] >>
-     Q.LIST_EXISTS_TAC [`next`, `lex_cenv`, `inverse_cenv`] >> 
+     qexists_tac `tagenv` >>
      fs [cenv_inv_def] >>
      rw []
-     >- metis_tac [FLOOKUP_SUBMAP]
      >- metis_tac [FLOOKUP_SUBMAP]
      >- (fs [has_exns_def] >>
          metis_tac [FLOOKUP_SUBMAP])
@@ -255,50 +240,50 @@ val v_to_i2_weakening = Q.prove (
      >- metis_tac []));
 
 val (result_to_i2_rules, result_to_i2_ind, result_to_i2_cases) = Hol_reln `
-(∀genv v v'. 
-  f genv v v'
+(∀gtagenv v v'. 
+  f gtagenv v v'
   ⇒
-  result_to_i2 f genv (Rval v) (Rval v')) ∧
-(∀genv v v'. 
-  v_to_i2 genv v v'
+  result_to_i2 f gtagenv (Rval v) (Rval v')) ∧
+(∀gtagenv v v'. 
+  v_to_i2 gtagenv v v'
   ⇒
-  result_to_i2 f genv (Rerr (Rraise v)) (Rerr (Rraise v'))) ∧
-(!genv.
-  result_to_i2 f genv (Rerr Rtimeout_error) (Rerr Rtimeout_error)) ∧
-(!genv.
-  result_to_i2 f genv (Rerr Rtype_error) (Rerr Rtype_error))`;
+  result_to_i2 f gtagenv (Rerr (Rraise v)) (Rerr (Rraise v'))) ∧
+(!gtagenv.
+  result_to_i2 f gtagenv (Rerr Rtimeout_error) (Rerr Rtimeout_error)) ∧
+(!gtagenv.
+  result_to_i2 f gtagenv (Rerr Rtype_error) (Rerr Rtype_error))`;
 
 val result_to_i2_eqns = Q.prove (
-`(!genv v r.
-  result_to_i2 f genv (Rval v) r ⇔ 
-    ?v'. f genv v v' ∧ r = Rval v') ∧
- (!genv v r.
-  result_to_i2 f genv (Rerr (Rraise v)) r ⇔ 
-    ?v'. v_to_i2 genv v v' ∧ r = Rerr (Rraise v')) ∧
- (!genv v r.
-  result_to_i2 f genv (Rerr Rtimeout_error) r ⇔ 
+`(!gtagenv v r.
+  result_to_i2 f gtagenv (Rval v) r ⇔ 
+    ?v'. f gtagenv v v' ∧ r = Rval v') ∧
+ (!gtagenv v r.
+  result_to_i2 f gtagenv (Rerr (Rraise v)) r ⇔ 
+    ?v'. v_to_i2 gtagenv v v' ∧ r = Rerr (Rraise v')) ∧
+ (!gtagenv v r.
+  result_to_i2 f gtagenv (Rerr Rtimeout_error) r ⇔ 
     r = Rerr Rtimeout_error) ∧
- (!genv v r.
-  result_to_i2 f genv (Rerr Rtype_error) r ⇔ 
+ (!gtagenv v r.
+  result_to_i2 f gtagenv (Rerr Rtype_error) r ⇔ 
     r = Rerr Rtype_error)`,
 rw [result_to_i2_cases] >>
 metis_tac []);
 
 val (s_to_i2'_rules, s_to_i2'_ind, s_to_i2'_cases) = Hol_reln `
-(!genv s s'.
-  vs_to_i2 genv s s'
+(!gtagenv s s'.
+  vs_to_i2 gtagenv s s'
   ⇒
-  s_to_i2' genv s s')`;
+  s_to_i2' gtagenv s s')`;
 
 val (s_to_i2_rules, s_to_i2_ind, s_to_i2_cases) = Hol_reln `
-(!genv c s s'.
-  s_to_i2' genv s s'
+(!gtagenv c s s'.
+  s_to_i2' gtagenv s s'
   ⇒
-  s_to_i2 genv (c,s) (c,s'))`;
+  s_to_i2 gtagenv (c,s) (c,s'))`;
 
 val length_vs_to_i2 = Q.prove (
-`!vs cenv vs'. 
-  vs_to_i2 cenv vs vs'
+`!vs gtagenv vs'. 
+  vs_to_i2 gtagenv vs vs'
   ⇒
   LENGTH vs = LENGTH vs'`,
  induct_on `vs` >>
@@ -307,8 +292,8 @@ val length_vs_to_i2 = Q.prove (
  metis_tac []);
 
 val length_evaluate_list_i2 = Q.prove (
-`!b env s cenv es s' vs.
-  evaluate_list_i2 b env s (exps_to_i2 cenv es) (s', Rval vs)
+`!b env s gtagenv es s' vs.
+  evaluate_list_i2 b env s (exps_to_i2 gtagenv es) (s', Rval vs)
   ⇒
   LENGTH es = LENGTH vs`,
  induct_on `es` >>
@@ -319,9 +304,9 @@ val length_evaluate_list_i2 = Q.prove (
  metis_tac []);
 
 val env_to_i2_el = Q.prove (
-`!cenv env env_i2. 
-  env_to_i2 cenv env env_i2 ⇔ 
-  LENGTH env = LENGTH env_i2 ∧ !n. n < LENGTH env ⇒ (FST (EL n env) = FST (EL n env_i2)) ∧ v_to_i2 cenv (SND (EL n env)) (SND (EL n env_i2))`,
+`!gtagenv env env_i2. 
+  env_to_i2 gtagenv env env_i2 ⇔ 
+  LENGTH env = LENGTH env_i2 ∧ !n. n < LENGTH env ⇒ (FST (EL n env) = FST (EL n env_i2)) ∧ v_to_i2 gtagenv (SND (EL n env)) (SND (EL n env_i2))`,
  induct_on `env` >>
  rw [v_to_i2_eqns]
  >- (cases_on `env_i2` >>
@@ -345,32 +330,31 @@ val env_to_i2_el = Q.prove (
      FIRST_X_ASSUM (qspecl_then [`SUC n`] mp_tac) >>
      rw []));
 
-
 val vs_to_i2_lupdate = Q.prove (
-`!cenv v n s v_i2 n s_i2.
-  vs_to_i2 cenv s s_i2 ∧
-  v_to_i2 cenv v v_i2
+`!gtagenv v n s v_i2 n s_i2.
+  vs_to_i2 gtagenv s s_i2 ∧
+  v_to_i2 gtagenv v v_i2
   ⇒
-  vs_to_i2 cenv (LUPDATE v n s) (LUPDATE v_i2 n s_i2)`,
+  vs_to_i2 gtagenv (LUPDATE v n s) (LUPDATE v_i2 n s_i2)`,
  induct_on `n` >>
  rw [v_to_i2_eqns, LUPDATE_def] >>
  cases_on `s` >>
  fs [v_to_i2_eqns, LUPDATE_def]);
 
 val match_result_to_i2_def = Define 
-`(match_result_to_i2 cenv (Match env) (Match env_i2) ⇔ 
-   env_to_i2 cenv env env_i2) ∧
- (match_result_to_i2 cenv No_match No_match = T) ∧
- (match_result_to_i2 cenv Match_type_error Match_type_error = T) ∧
- (match_result_to_i2 cenv _ _ = F)`;
+`(match_result_to_i2 gtagenv (Match env) (Match env_i2) ⇔ 
+   env_to_i2 gtagenv env env_i2) ∧
+ (match_result_to_i2 gtagenv No_match No_match = T) ∧
+ (match_result_to_i2 gtagenv Match_type_error Match_type_error = T) ∧
+ (match_result_to_i2 gtagenv _ _ = F)`;
 
 val store_lookup_vs_to_i2 = Q.prove (
-`!cenv vs vs_i2 v v_i2 n.
-  vs_to_i2 cenv vs vs_i2 ∧
+`!gtagenv vs vs_i2 v v_i2 n.
+  vs_to_i2 gtagenv vs vs_i2 ∧
   store_lookup n vs = SOME v ∧
   store_lookup n vs_i2 = SOME v_i2
   ⇒
-  v_to_i2 cenv v v_i2`,
+  v_to_i2 gtagenv v v_i2`,
  induct_on `vs` >>
  rw [v_to_i2_eqns] >>
  fs [store_lookup_def] >>
@@ -379,8 +363,8 @@ val store_lookup_vs_to_i2 = Q.prove (
  metis_tac []);
 
 val store_lookup_vs_to_i2_2 = Q.prove (
-`!cenv vs vs_i2 v v_i2 n.
-  vs_to_i2 cenv vs vs_i2 ∧
+`!gtagenv vs vs_i2 v v_i2 n.
+  vs_to_i2 gtagenv vs vs_i2 ∧
   store_lookup n vs = SOME v
   ⇒
   ?v'. store_lookup n vs_i2 = SOME v'`,
@@ -404,7 +388,7 @@ val pat_bindings_i2_accum = Q.store_thm ("pat_bindings_ai2_ccum",
  >- metis_tac [APPEND_ASSOC, pat_bindings_i2_def]);
 
 val pat_bindings_to_i2 = Q.prove (
-`!cenv p x. pat_bindings_i2 (pat_to_i2 cenv p) x = pat_bindings p x`,
+`!tagenv p x. pat_bindings_i2 (pat_to_i2 tagenv p) x = pat_bindings p x`,
  ho_match_mp_tac pat_to_i2_ind >>
  rw [pat_bindings_def, pat_bindings_i2_def, pat_to_i2_def] >>
  induct_on `ps` >>
@@ -413,28 +397,28 @@ val pat_bindings_to_i2 = Q.prove (
  metis_tac [APPEND_11, pat_bindings_accum, pat_bindings_i2_accum]);
 
 val pmatch_to_i2_correct = Q.prove (
-`(!envC s p v env r env_i2 s_i2 v_i2 next lex_cenv cenv inverse_cenv clengths.
+`(!envC s p v env r env_i2 s_i2 v_i2 tagenv gtagenv.
   r ≠ Match_type_error ∧
-  cenv_inv envC (next,lex_cenv,cenv,inverse_cenv) clengths ∧
+  cenv_inv envC tagenv gtagenv ∧
   pmatch_i1 envC s p v env = r ∧
-  s_to_i2' (cenv,clengths) s s_i2 ∧
-  v_to_i2 (cenv,clengths) v v_i2 ∧
-  env_to_i2 (cenv,clengths) env env_i2
+  s_to_i2' gtagenv s s_i2 ∧
+  v_to_i2 gtagenv v v_i2 ∧
+  env_to_i2 gtagenv env env_i2
   ⇒
   ?r_i2.
-    pmatch_i2 s_i2 (pat_to_i2 lex_cenv p) v_i2 env_i2 = r_i2 ∧
-    match_result_to_i2 (cenv,clengths) r r_i2) ∧
- (!envC s ps vs env r env_i2 s_i2 vs_i2 next lex_cenv cenv inverse_cenv clengths.
+    pmatch_i2 s_i2 (pat_to_i2 tagenv p) v_i2 env_i2 = r_i2 ∧
+    match_result_to_i2 gtagenv r r_i2) ∧
+ (!envC s ps vs env r env_i2 s_i2 vs_i2 tagenv gtagenv.
   r ≠ Match_type_error ∧
-  cenv_inv envC (next,lex_cenv,cenv,inverse_cenv) clengths ∧
+  cenv_inv envC tagenv gtagenv ∧
   pmatch_list_i1 envC s ps vs env = r ∧
-  s_to_i2' (cenv,clengths) s s_i2 ∧
-  vs_to_i2 (cenv,clengths) vs vs_i2 ∧
-  env_to_i2 (cenv,clengths) env env_i2
+  s_to_i2' gtagenv s s_i2 ∧
+  vs_to_i2 gtagenv vs vs_i2 ∧
+  env_to_i2 gtagenv env env_i2
   ⇒
   ?r_i2.
-    pmatch_list_i2 s_i2 (MAP (pat_to_i2 lex_cenv) ps) vs_i2 env_i2 = r_i2 ∧
-    match_result_to_i2 (cenv,clengths) r r_i2)`,
+    pmatch_list_i2 s_i2 (MAP (pat_to_i2 tagenv) ps) vs_i2 env_i2 = r_i2 ∧
+    match_result_to_i2 gtagenv r r_i2)`,
  ho_match_mp_tac pmatch_i1_ind >>
  rw [pmatch_i1_def, pmatch_i2_def, pat_to_i2_def, match_result_to_i2_def] >>
  fs [match_result_to_i2_def, bind_def, v_to_i2_eqns] >>
@@ -444,30 +428,30 @@ val pmatch_to_i2_correct = Q.prove (
      every_case_tac >>
      fs [] 
      >- metis_tac [] >>
-     fs [lookup_tag_def, cenv_inv_def] >>
+     fs [cenv_inv_def] >>
      res_tac >>
      fs [] >>
      rw [] >>
      imp_res_tac same_tid_diff_ctor >>
      rw [] >>
-     metis_tac [tid_or_exn_11])
+     metis_tac [tid_or_exn_11, SOME_11, PAIR_EQ])
  >- (cases_on `lookup_con_id n envC` >>
      fs [] >>
      every_case_tac >>
      fs [] >> 
      rw []
-     >- metis_tac [length_vs_to_i2, cenv_inv_def, SOME_11, same_ctor_and_same_tid] >>
-     fs [lookup_tag_def, cenv_inv_def] >>
+     >- metis_tac [length_vs_to_i2, cenv_inv_def, SOME_11, same_ctor_and_same_tid, PAIR_EQ] >>
+     fs [cenv_inv_def] >>
      res_tac >>
      fs [] >>
      rw [] >>
      imp_res_tac same_tid_diff_ctor >>
      rw [] >>
-     metis_tac [tid_or_exn_11])
+     metis_tac [tid_or_exn_11, SOME_11, PAIR_EQ])
  >- (cases_on `lookup_con_id n envC` >>
      fs [] >>
      every_case_tac >>
-     fs [lookup_tag_def, cenv_inv_def] >>
+     fs [cenv_inv_def] >>
      imp_res_tac same_ctor_and_same_tid >>
      imp_res_tac same_tid_diff_ctor >>
      rw [] >>
@@ -475,7 +459,8 @@ val pmatch_to_i2_correct = Q.prove (
      fs [match_result_to_i2_def])
  >- metis_tac []
  >- metis_tac [length_vs_to_i2]
- >- fs [lookup_tag_def]
+ >- (PairCases_on `tagenv` >>
+     fs [lookup_tag_env_def])
  >- (every_case_tac >>
      fs [s_to_i2'_cases] >>
      imp_res_tac store_lookup_vs_to_i2 >>
@@ -493,31 +478,31 @@ val pmatch_to_i2_correct = Q.prove (
      metis_tac [match_result_to_i2_def, match_result_distinct]));
 
 val (env_all_to_i2_rules, env_all_to_i2_ind, env_all_to_i2_cases) = Hol_reln `
-(!genv envC clengths lex_cenv next cenv inverse_cenv env env_i2 genv_i2.
-  cenv_inv envC (next, lex_cenv, cenv, inverse_cenv) clengths ∧
-  vs_to_i2 (cenv,clengths) genv genv_i2 ∧
-  env_to_i2 (cenv,clengths) env env_i2
+(!genv envC gtagenv env env_i2 genv_i2.
+  cenv_inv envC tagenv gtagenv ∧
+  vs_to_i2 gtagenv genv genv_i2 ∧
+  env_to_i2 gtagenv env env_i2
   ⇒
-  env_all_to_i2 (next, lex_cenv, cenv, inverse_cenv) (genv,envC,env) (genv_i2,env_i2) (cenv,clengths))`;
+  env_all_to_i2 tagenv (genv,envC,env) (genv_i2,env_i2) gtagenv)`;
 
 val env_to_i2_append = Q.prove (
-`!cenv env1 env2 env1' env2'.
-  env_to_i2 cenv env1 env1' ∧
-  env_to_i2 cenv env2 env2' 
+`!gtagenv env1 env2 env1' env2'.
+  env_to_i2 gtagenv env1 env1' ∧
+  env_to_i2 gtagenv env2 env2' 
   ⇒
-  env_to_i2 cenv (env1++env2) (env1'++env2')`,
+  env_to_i2 gtagenv (env1++env2) (env1'++env2')`,
  induct_on `env1` >>
  rw [v_to_i2_eqns] >>
  PairCases_on `h` >>
  fs [v_to_i2_eqns]);
 
 val env_to_i2_lookup = Q.prove (
-`!cenv env x v env'.
+`!gtagenv env x v env'.
   lookup x env = SOME v ∧
-  env_to_i2 cenv env env'
+  env_to_i2 gtagenv env env'
   ⇒
   ?v'.
-    v_to_i2 cenv v v' ∧
+    v_to_i2 gtagenv v v' ∧
     lookup x env' = SOME v'`,
  induct_on `env` >>
  rw [] >>
@@ -529,22 +514,22 @@ val env_to_i2_lookup = Q.prove (
  fs [v_to_i2_eqns]);
 
 val genv_to_i2_lookup = Q.prove (
-`!cenv genv n genv'.
-  vs_to_i2 cenv genv genv' ∧
+`!gtagenv genv n genv'.
+  vs_to_i2 gtagenv genv genv' ∧
   LENGTH genv > n
   ⇒
-  v_to_i2 cenv (EL n genv) (EL n genv')`,
+  v_to_i2 gtagenv (EL n genv) (EL n genv')`,
  induct_on `genv` >>
  srw_tac [ARITH_ss] [v_to_i2_eqns] >>
  cases_on `n` >>
  srw_tac [ARITH_ss] [v_to_i2_eqns]);
 
 val vs_to_i2_append1 = Q.prove (
-`!cenv vs v vs' v'.
-  vs_to_i2 cenv (vs++[v]) (vs'++[v'])
+`!gtagenv vs v vs' v'.
+  vs_to_i2 gtagenv (vs++[v]) (vs'++[v'])
   ⇔
-  vs_to_i2 cenv vs vs' ∧
-  v_to_i2 cenv v v'`,
+  vs_to_i2 gtagenv vs vs' ∧
+  v_to_i2 gtagenv v v'`,
  induct_on `vs` >>
  rw [] >>
  cases_on `vs'` >>
@@ -554,11 +539,11 @@ val vs_to_i2_append1 = Q.prove (
  metis_tac []);
 
 val vs_to_i2_append = Q.prove (
-`!cenv vs1 vs1' vs2 vs2'.
+`!gtagenv vs1 vs1' vs2 vs2'.
   (LENGTH vs2 = LENGTH vs2' ∨ LENGTH vs1 = LENGTH vs1')
   ⇒
-  (vs_to_i2 cenv (vs1++vs2) (vs1'++vs2') ⇔
-   vs_to_i2 cenv vs1 vs1' ∧ vs_to_i2 cenv vs2 vs2')`,
+  (vs_to_i2 gtagenv (vs1++vs2) (vs1'++vs2') ⇔
+   vs_to_i2 gtagenv vs1 vs1' ∧ vs_to_i2 gtagenv vs2 vs2')`,
  induct_on `vs1` >>
  rw [v_to_i2_eqns] >>
  eq_tac >>
@@ -572,14 +557,14 @@ val vs_to_i2_append = Q.prove (
  metis_tac []);
 
 val do_uapp_correct = Q.prove (
-`!s uop v s' v' cenv s_i2 v_i2.
+`!s uop v s' v' gtagenv s_i2 v_i2.
   do_uapp_i1 s uop v = SOME (s',v') ∧
-  s_to_i2' cenv s s_i2 ∧
-  v_to_i2 cenv v v_i2
+  s_to_i2' gtagenv s s_i2 ∧
+  v_to_i2 gtagenv v v_i2
   ⇒
   ∃s'_i2 v'_i2.
-    s_to_i2' cenv s' s'_i2 ∧
-    v_to_i2 cenv v' v'_i2 ∧
+    s_to_i2' gtagenv s' s'_i2 ∧
+    v_to_i2 gtagenv v' v'_i2 ∧
     do_uapp_i2 s_i2 uop v_i2 = SOME (s'_i2,v'_i2)`,
  cases_on `uop` >>
  rw [do_uapp_i1_def, do_uapp_i2_def, LET_THM, store_alloc_def, s_to_i2'_cases] >>
@@ -591,35 +576,35 @@ val do_uapp_correct = Q.prove (
  >- metis_tac [store_lookup_vs_to_i2]);
 
 val exn_env_i2_correct = Q.prove (
-`!cenv cenv'.
-  env_all_to_i2 (next,lex_cenv,type_cenv,inverse_cenv) env env_i2 cenv'
+`!gtagenv.
+  env_all_to_i2 tagenv env env_i2 gtagenv
   ⇒
-  env_all_to_i2 (next,FST (SND init_cenv_mapping),type_cenv,inverse_cenv) (exn_env_i1 (all_env_i1_to_genv env))
-    (exn_env_i2 (all_env_i2_to_genv env_i2)) cenv'`,
+  env_all_to_i2 (FST (SND init_tagenv_state)) (exn_env_i1 (all_env_i1_to_genv env))
+    (exn_env_i2 (all_env_i2_to_genv env_i2)) gtagenv`,
  rw [env_all_to_i2_cases, exn_env_i1_def, exn_env_i2_def, emp_def, v_to_i2_eqns,
-     all_env_i1_to_genv_def, all_env_i2_to_genv_def, init_cenv_mapping_def] >>
+     all_env_i1_to_genv_def, all_env_i2_to_genv_def, init_tagenv_state_def] >>
  fs [cenv_inv_def, lookup_con_id_def] >>
  rw [] >>
  every_case_tac >>
  fs [] >>
  rw [id_to_n_def] >>
  fs [has_exns_def] >>
- fs [flookup_fupdate_list] >>
+ fs [flookup_fupdate_list, lookup_tag_env_def, lookup_tag_flat_def, all_env_i1_to_genv_def, all_env_i2_to_genv_def] >>
  metis_tac []);
 
 val do_eq_i2 = Q.prove (
-`(!v1 v2 cenv r v1_i2 v2_i2 cenv'.
-  env_all_to_i2 cenv env env_i2 cenv' ∧
+`(!v1 v2 tagenv r v1_i2 v2_i2 gtagenv.
+  env_all_to_i2 tagenv env env_i2 gtagenv ∧
   do_eq_i1 v1 v2 = r ∧
-  v_to_i2 cenv' v1 v1_i2 ∧
-  v_to_i2 cenv' v2 v2_i2
+  v_to_i2 gtagenv v1 v1_i2 ∧
+  v_to_i2 gtagenv v2 v2_i2
   ⇒ 
   do_eq_i2 v1_i2 v2_i2 = r) ∧
- (!vs1 vs2 cenv r vs1_i2 vs2_i2 cenv'.
-  env_all_to_i2 cenv env env_i2 cenv' ∧
+ (!vs1 vs2 tagenv r vs1_i2 vs2_i2 gtagenv.
+  env_all_to_i2 tagenv env env_i2 gtagenv ∧
   do_eq_list_i1 vs1 vs2 = r ∧
-  vs_to_i2 cenv' vs1 vs1_i2 ∧
-  vs_to_i2 cenv' vs2 vs2_i2
+  vs_to_i2 gtagenv vs1 vs1_i2 ∧
+  vs_to_i2 gtagenv vs2 vs2_i2
   ⇒ 
   do_eq_list_i2 vs1_i2 vs2_i2 = r)`,
  ho_match_mp_tac do_eq_i1_ind >>
@@ -632,10 +617,10 @@ val do_eq_i2 = Q.prove (
  >- metis_tac []
  >- metis_tac []
  >- metis_tac []
- >- metis_tac [cenv_inv_def]
- >- metis_tac [cenv_inv_def]
- >- metis_tac [cenv_inv_def]
- >- metis_tac [cenv_inv_def]
+ >- metis_tac [cenv_inv_def, SOME_11, PAIR_EQ, pair_CASES]
+ >- metis_tac [cenv_inv_def, SOME_11, PAIR_EQ, pair_CASES]
+ >- metis_tac [cenv_inv_def, SOME_11, PAIR_EQ, pair_CASES]
+ >- metis_tac [cenv_inv_def, SOME_11, PAIR_EQ, pair_CASES]
  >- (fs [Once v_to_i2_cases] >>
      rw [do_eq_i2_def])
  >- (fs [Once v_to_i2_cases] >>
@@ -682,17 +667,17 @@ val do_eq_i2 = Q.prove (
  metis_tac []);
 
 val do_app_i2_correct = Q.prove (
-`!env s op v1 v2 s' e env' cenv s_i2 v1_i2 v2_i2 env_i2 cenv'.
+`!env s op v1 v2 s' e env' tagenv s_i2 v1_i2 v2_i2 env_i2 gtagenv.
   do_app_i1 env s op v1 v2 = SOME (env',s',e) ∧
-  env_all_to_i2 cenv env env_i2 cenv' ∧
-  s_to_i2' cenv' s s_i2 ∧
-  v_to_i2 cenv' v1 v1_i2 ∧
-  v_to_i2 cenv' v2 v2_i2
+  env_all_to_i2 tagenv env env_i2 gtagenv ∧
+  s_to_i2' gtagenv s s_i2 ∧
+  v_to_i2 gtagenv v1 v1_i2 ∧
+  v_to_i2 gtagenv v2 v2_i2
   ⇒
-  ∃s'_i2 env'_i2 cenv.
-    env_all_to_i2 cenv env' env'_i2 cenv' ∧
-    s_to_i2' cenv' s' s'_i2 ∧
-    do_app_i2 env_i2 s_i2 op v1_i2 v2_i2 = SOME (env'_i2,s'_i2,exp_to_i2 (cenv_mapping_to_lex_cenv cenv) e)`,
+  ∃s'_i2 env'_i2 tagenv'.
+    env_all_to_i2 tagenv' env' env'_i2 gtagenv ∧
+    s_to_i2' gtagenv s' s'_i2 ∧
+    do_app_i2 env_i2 s_i2 op v1_i2 v2_i2 = SOME (env'_i2,s'_i2,exp_to_i2 tagenv' e)`,
  cases_on `op` >>
  rw [do_app_i1_def, do_app_i2_def]
  >- (cases_on `v2` >>
@@ -704,17 +689,15 @@ val do_app_i2_correct = Q.prove (
      fs [] >>
      rw [] >>
      fs [v_to_i2_eqns] >>
-     rw [exp_to_i2_def] >>
-     `?next lex_cenv type_cenv inverse_cenv. cenv = (next,lex_cenv,type_cenv,inverse_cenv)` by metis_tac [pair_CASES] >>
-     rw []
-     >- (qexists_tac `(next,FST (SND init_cenv_mapping),type_cenv,inverse_cenv)` >>
+     rw [exp_to_i2_def]
+     >- (qexists_tac `FST (SND init_tagenv_state)` >>
          rw []
          >- metis_tac [exn_env_i2_correct]
-         >- rw [init_cenv_mapping_def, flookup_fupdate_list, lookup_tag_def, cenv_mapping_to_lex_cenv_def])
-     >- (qexists_tac `(next,FST (SND init_cenv_mapping),type_cenv,inverse_cenv)` >>
+         >- rw [init_tagenv_state_def, flookup_fupdate_list, lookup_tag_env_def, lookup_tag_flat_def])
+     >- (qexists_tac `FST (SND init_tagenv_state)` >>
          rw []
          >- metis_tac [exn_env_i2_correct]
-         >- rw [init_cenv_mapping_def, flookup_fupdate_list, lookup_tag_def, cenv_mapping_to_lex_cenv_def])
+         >- rw [init_tagenv_state_def, flookup_fupdate_list, lookup_tag_env_def, lookup_tag_flat_def])
      >- metis_tac []
      >- metis_tac [])
  >- (cases_on `v2` >>
@@ -733,22 +716,20 @@ val do_app_i2_correct = Q.prove (
      >- metis_tac [do_eq_i2, eq_result_11, eq_result_distinct]
      >- metis_tac [do_eq_i2, eq_result_11, eq_result_distinct]
      >- metis_tac [do_eq_i2, eq_result_11, eq_result_distinct]
-     >- (`?next lex_cenv type_cenv inverse_cenv. cenv = (next,lex_cenv,type_cenv,inverse_cenv)` by metis_tac [pair_CASES] >>
-         rw [] >>
-         qexists_tac `(next,FST (SND init_cenv_mapping),type_cenv,inverse_cenv)` >>
+     >- (qexists_tac `FST (SND init_tagenv_state)` >>
          rw []
          >- metis_tac [exn_env_i2_correct]
-         >- rw [init_cenv_mapping_def, flookup_fupdate_list, lookup_tag_def, cenv_mapping_to_lex_cenv_def])
+         >- rw [init_tagenv_state_def, flookup_fupdate_list, lookup_tag_env_def, lookup_tag_flat_def])
      >- metis_tac [do_eq_i2, eq_result_11, eq_result_distinct]
      >- metis_tac [do_eq_i2, eq_result_11, eq_result_distinct])
  >- (every_case_tac >>
      fs [] >>
      pop_assum (mp_tac o SIMP_RULE (srw_ss()) [Once v_to_i2_cases]) >>
      rw []
-     >- (qexists_tac `(next,lex_cenv,cenv'',inverse_cenv)` >>
+     >- (qexists_tac `tagenv'` >>
          rw [] >>
          fs [env_all_to_i2_cases, bind_def] >>
-         rw [v_to_i2_eqns, all_env_i1_to_genv_def, all_env_i2_to_genv_def, cenv_mapping_to_lex_cenv_def])
+         rw [v_to_i2_eqns, all_env_i1_to_genv_def, all_env_i2_to_genv_def, get_tagenv_def])
      >- (CCONTR_TAC >>
          fs [] >>
          rw [] >>
@@ -759,7 +740,7 @@ val do_app_i2_correct = Q.prove (
          fs [exp_to_i2_def] >>
          every_case_tac >>
          fs [])
-     >- (qexists_tac `(next,lex_cenv,cenv'',inverse_cenv)` >>
+     >- (qexists_tac `tagenv'` >>
          rw [] >>
          fs [env_all_to_i2_cases, bind_def] >>
          rw [v_to_i2_eqns, all_env_i1_to_genv_def, all_env_i2_to_genv_def, 
@@ -785,7 +766,7 @@ val do_app_i2_correct = Q.prove (
              PairCases_on `h` >>
              fs [exp_to_i2_def] >>
              every_case_tac >>
-             fs [cenv_mapping_to_lex_cenv_def])))
+             fs [get_tagenv_def])))
  >- (every_case_tac >>
      fs [] >>
      rw [] >>
@@ -794,47 +775,52 @@ val do_app_i2_correct = Q.prove (
      rw [exp_to_i2_def, s_to_i2'_cases] >>
      metis_tac [vs_to_i2_lupdate, s_to_i2'_cases]));
 
+val lookup_tag_env_NONE = Q.prove (
+`lookup_tag_env NONE tagenv = tuple_tag`,
+PairCases_on `tagenv` >>
+rw [lookup_tag_env_def]);
+
 val exp_to_i2_correct = Q.prove (
 `(∀b env s e res. 
    evaluate_i1 b env s e res ⇒ 
    (SND res ≠ Rerr Rtype_error) ⇒
-   !cenv s' r env_i2 s_i2 e_i2 cenv'.
+   !tagenv s' r env_i2 s_i2 e_i2 gtagenv.
      (res = (s',r)) ∧
-     env_all_to_i2 cenv env env_i2 cenv' ∧
-     s_to_i2 cenv' s s_i2 ∧
-     (e_i2 = exp_to_i2 (cenv_mapping_to_lex_cenv cenv) e)
+     env_all_to_i2 tagenv env env_i2 gtagenv ∧
+     s_to_i2 gtagenv s s_i2 ∧
+     (e_i2 = exp_to_i2 tagenv e)
      ⇒
      ∃s'_i2 r_i2.
-       result_to_i2 v_to_i2 cenv' r r_i2 ∧
-       s_to_i2 cenv' s' s'_i2 ∧
+       result_to_i2 v_to_i2 gtagenv r r_i2 ∧
+       s_to_i2 gtagenv s' s'_i2 ∧
        evaluate_i2 b env_i2 s_i2 e_i2 (s'_i2, r_i2)) ∧
  (∀b env s es res.
    evaluate_list_i1 b env s es res ⇒ 
    (SND res ≠ Rerr Rtype_error) ⇒
-   !cenv s' r env_i2 s_i2 es_i2 cenv'.
+   !tagenv s' r env_i2 s_i2 es_i2 gtagenv.
      (res = (s',r)) ∧
-     env_all_to_i2 cenv env env_i2 cenv' ∧
-     s_to_i2 cenv' s s_i2 ∧
-     (es_i2 = exps_to_i2 (cenv_mapping_to_lex_cenv cenv) es)
+     env_all_to_i2 tagenv env env_i2 gtagenv ∧
+     s_to_i2 gtagenv s s_i2 ∧
+     (es_i2 = exps_to_i2 tagenv es)
      ⇒
      ?s'_i2 r_i2.
-       result_to_i2 vs_to_i2 cenv' r r_i2 ∧
-       s_to_i2 cenv' s' s'_i2 ∧
+       result_to_i2 vs_to_i2 gtagenv r r_i2 ∧
+       s_to_i2 gtagenv s' s'_i2 ∧
        evaluate_list_i2 b env_i2 s_i2 es_i2 (s'_i2, r_i2)) ∧
  (∀b env s v pes err_v res. 
    evaluate_match_i1 b env s v pes err_v res ⇒ 
    (SND res ≠ Rerr Rtype_error) ⇒
-   !cenv s' r env_i2 s_i2 v_i2 pes_i2 err_v_i2 cenv'.
+   !tagenv s' r env_i2 s_i2 v_i2 pes_i2 err_v_i2 gtagenv.
      (res = (s',r)) ∧
-     env_all_to_i2 cenv env env_i2 cenv' ∧
-     s_to_i2 cenv' s s_i2 ∧
-     v_to_i2 cenv' v v_i2 ∧
-     (pes_i2 = pat_exp_to_i2 (cenv_mapping_to_lex_cenv cenv) pes) ∧
-     v_to_i2 cenv' err_v err_v_i2
+     env_all_to_i2 tagenv env env_i2 gtagenv ∧
+     s_to_i2 gtagenv s s_i2 ∧
+     v_to_i2 gtagenv v v_i2 ∧
+     (pes_i2 = pat_exp_to_i2 tagenv pes) ∧
+     v_to_i2 gtagenv err_v err_v_i2
      ⇒
      ?s'_i2 r_i2.
-       result_to_i2 v_to_i2 cenv' r r_i2 ∧
-       s_to_i2 cenv' s' s'_i2 ∧
+       result_to_i2 v_to_i2 gtagenv r r_i2 ∧
+       s_to_i2 gtagenv s' s'_i2 ∧
        evaluate_match_i2 b env_i2 s_i2 v_i2 pes_i2 err_v_i2 (s'_i2, r_i2))`,
  ho_match_mp_tac evaluate_i1_ind >>
  rw [] >>
@@ -851,23 +837,18 @@ val exp_to_i2_correct = Q.prove (
      rw [] >>
      fs [env_all_to_i2_cases, build_conv_i1_def] >>
      rw [] >>
-     MAP_EVERY qexists_tac [`s'_i2`, `Rval (Conv_i2 (lookup_tag cn lex_cenv) v')`] >>
+     MAP_EVERY qexists_tac [`s'_i2`, `Rval (Conv_i2 (lookup_tag_env cn tagenv) v')`] >>
      rw [] >>
      Cases_on `cn` >>
      fs [] >>
-     rw [v_to_i2_eqns, lookup_tag_def] >>
+     rw [v_to_i2_eqns, lookup_tag_env_NONE] >>
      fs [all_env_i1_to_cenv_def] >>
      every_case_tac >>
-     fs [cenv_mapping_to_lex_cenv_def] >>
-     rw [v_to_i2_eqns]
-     >- metis_tac [NOT_SOME_NONE, cenv_inv_def]
-     >- metis_tac [NOT_SOME_NONE, cenv_inv_def]
-     >- metis_tac [NOT_SOME_NONE, cenv_inv_def]
-     >- metis_tac [NOT_SOME_NONE, cenv_inv_def]
-     >- (fs [cenv_inv_def, do_con_check_def] >>
-         rw [] >>
-         metis_tac [length_evaluate_list_i2, length_vs_to_i2])
-     >- metis_tac [NOT_SOME_NONE, cenv_inv_def])
+     fs [get_tagenv_def] >>
+     rw [v_to_i2_eqns] >>
+     fs [cenv_inv_def, do_con_check_def] >>
+     rw [] >>
+     metis_tac [length_evaluate_list_i2, length_vs_to_i2])
  >- metis_tac []
  >- (* Local variable lookup *)
     (fs [env_all_to_i2_cases, all_env_i2_to_env_def] >>
@@ -881,7 +862,7 @@ val exp_to_i2_correct = Q.prove (
      metis_tac [genv_to_i2_lookup, length_vs_to_i2])
  >- (rw [Once v_to_i2_cases] >>
      fs [env_all_to_i2_cases] >>
-     rw [all_env_i1_to_env_def, all_env_i2_to_env_def, all_env_i1_to_cenv_def, cenv_mapping_to_lex_cenv_def] >>
+     rw [all_env_i1_to_env_def, all_env_i2_to_env_def, all_env_i1_to_cenv_def] >>
      metis_tac [])
  >- (* Uapp *)
     (res_tac >>
@@ -889,35 +870,35 @@ val exp_to_i2_correct = Q.prove (
      fs [s_to_i2_cases] >>
      rw [] >>
      `?s3_i2 v'_i2. do_uapp_i2 s''' uop v'' = SOME (s3_i2, v'_i2) ∧
-       s_to_i2' cenv' s3 s3_i2 ∧ v_to_i2 cenv' v' v'_i2` by metis_tac [do_uapp_correct] >>
+       s_to_i2' gtagenv s3 s3_i2 ∧ v_to_i2 gtagenv v' v'_i2` by metis_tac [do_uapp_correct] >>
      metis_tac [])
  >- metis_tac []
  >- (* App *)
-    (LAST_X_ASSUM (qspecl_then [`cenv`, `env_i2`, `s_i2`, `cenv'`] mp_tac) >>
+    (LAST_X_ASSUM (qspecl_then [`tagenv`, `env_i2`, `s_i2`, `gtagenv`] mp_tac) >>
      rw [] >>
-     LAST_X_ASSUM (qspecl_then [`cenv`, `env_i2`, `s'_i2`, `cenv'`] mp_tac) >>
-     rw [] >>
-     fs [s_to_i2_cases] >>
-     rw [] >>
-     (qspecl_then [`env`, `s3`, `op`, `v1`, `v2`, `s4`, `e''`, `env'`,
-                   `cenv`, `s'''''''`, `v'`, `v''`, `env_i2`, `cenv'`] mp_tac) do_app_i2_correct >>
-     rw [] >>
-     metis_tac [])
- >- (* App *)
-    (LAST_X_ASSUM (qspecl_then [`cenv`, `env_i2`, `s_i2`, `cenv'`] mp_tac) >>
-     rw [] >>
-     LAST_X_ASSUM (qspecl_then [`cenv`, `env_i2`, `s'_i2`, `cenv'`] mp_tac) >>
+     LAST_X_ASSUM (qspecl_then [`tagenv`, `env_i2`, `s'_i2`, `gtagenv`] mp_tac) >>
      rw [] >>
      fs [s_to_i2_cases] >>
      rw [] >>
      (qspecl_then [`env`, `s3`, `op`, `v1`, `v2`, `s4`, `e''`, `env'`,
-                   `cenv`, `s'''''''`, `v'`, `v''`, `env_i2`, `cenv'`] mp_tac) do_app_i2_correct >>
+                   `tagenv`, `s'''''''`, `v'`, `v''`, `env_i2`, `gtagenv`] mp_tac) do_app_i2_correct >>
      rw [] >>
      metis_tac [])
  >- (* App *)
-    (LAST_X_ASSUM (qspecl_then [`cenv`, `env_i2`, `s_i2`, `cenv'`] mp_tac) >>
+    (LAST_X_ASSUM (qspecl_then [`tagenv`, `env_i2`, `s_i2`, `gtagenv`] mp_tac) >>
      rw [] >>
-     LAST_X_ASSUM (qspecl_then [`cenv`, `env_i2`, `s'_i2`, `cenv'`] mp_tac) >>
+     LAST_X_ASSUM (qspecl_then [`tagenv`, `env_i2`, `s'_i2`, `gtagenv`] mp_tac) >>
+     rw [] >>
+     fs [s_to_i2_cases] >>
+     rw [] >>
+     (qspecl_then [`env`, `s3`, `op`, `v1`, `v2`, `s4`, `e''`, `env'`,
+                   `tagenv`, `s'''''''`, `v'`, `v''`, `env_i2`, `gtagenv`] mp_tac) do_app_i2_correct >>
+     rw [] >>
+     metis_tac [])
+ >- (* App *)
+    (LAST_X_ASSUM (qspecl_then [`tagenv`, `env_i2`, `s_i2`, `gtagenv`] mp_tac) >>
+     rw [] >>
+     LAST_X_ASSUM (qspecl_then [`tagenv`, `env_i2`, `s'_i2`, `gtagenv`] mp_tac) >>
      rw [] >>
      fs [s_to_i2_cases] >>
      rw [] >>
@@ -949,11 +930,12 @@ val exp_to_i2_correct = Q.prove (
     (pop_assum mp_tac >>
      res_tac >>
      rw [] >>
-     FIRST_X_ASSUM (qspecl_then [`cenv`, `env_i2`, `s'_i2'`, `v''`, `Conv_i2 bind_tag []`, `cenv'` ] mp_tac) >>
+     FIRST_X_ASSUM (qspecl_then [`tagenv`, `env_i2`, `s'_i2'`, `v''`, `Conv_i2 bind_tag []`, `gtagenv` ] mp_tac) >>
      rw [] >>
      fs [env_all_to_i2_cases] >>
      rw [] >>
      fs [cenv_inv_def, has_exns_def] >>
+     pop_assum (fn _ => all_tac) >>
      pop_assum mp_tac >>
      rw [] >>
      MAP_EVERY qexists_tac [`s'_i2''`, `r_i2`] >>
@@ -967,7 +949,7 @@ val exp_to_i2_correct = Q.prove (
      res_tac >>
      fs [] >>
      rw [] >>
-     `env_all_to_i2 cenv' (genv,cenv,bind n v env) (genv', (n,v')::env') cenv''`
+     `env_all_to_i2 tagenv (genv,cenv,bind n v env) (genv', (n,v')::env') gtagenv`
                 by (fs [env_all_to_i2_cases] >>
                     fs [bind_def, v_to_i2_eqns] >>
                     rw []) >>
@@ -979,13 +961,13 @@ val exp_to_i2_correct = Q.prove (
      rw [] >>
      `?genv' env'. env_i2 = (genv',env')` by metis_tac [pair_CASES] >>
      rw [] >>
-     `env_all_to_i2 cenv' (genv,cenv,build_rec_env_i1 funs (cenv,env) env) 
-                          (genv',build_rec_env_i2 (funs_to_i2 (cenv_mapping_to_lex_cenv cenv') funs) env' env') 
-                          cenv''`
+     `env_all_to_i2 tagenv (genv,cenv,build_rec_env_i1 funs (cenv,env) env) 
+                           (genv',build_rec_env_i2 (funs_to_i2 tagenv funs) env' env') 
+                           gtagenv`
          by (fs [env_all_to_i2_cases] >>
              rw [build_rec_env_i1_merge, build_rec_env_i2_merge, merge_def] >>
              match_mp_tac env_to_i2_append >>
-             rw [cenv_mapping_to_lex_cenv_def] >>
+             rw [] >>
              rw [funs_to_i2_map, MAP_MAP_o, combinTheory.o_DEF, LAMBDA_PROD, env_to_i2_el, EL_MAP] >>
              `?f x e. EL n funs = (f,x,e)` by metis_tac [pair_CASES] >>
              rw [] >>
@@ -1005,37 +987,31 @@ val exp_to_i2_correct = Q.prove (
      rw [] >>
      fs [s_to_i2_cases, env_all_to_i2_cases] >>
      rw [] >>
-     `match_result_to_i2 (cenv''',clengths) (Match env') 
-            (pmatch_i2 s'' (pat_to_i2 lex_cenv p) v_i2 env_i2')`
+     `match_result_to_i2 gtagenv (Match env') 
+            (pmatch_i2 s'' (pat_to_i2 tagenv p) v_i2 env_i2')`
                    by metis_tac [pmatch_to_i2_correct, match_result_distinct] >>
-     cases_on `pmatch_i2 s'' (pat_to_i2 lex_cenv p) v_i2 env_i2'` >>
+     cases_on `pmatch_i2 s'' (pat_to_i2 tagenv p) v_i2 env_i2'` >>
      fs [match_result_to_i2_def] >>
      rw [] >>
      fs [METIS_PROVE [] ``(((?x. P x) ∧ R ⇒ Q) ⇔ !x. P x ∧ R ⇒ Q) ∧ ((R ∧ (?x. P x) ⇒ Q) ⇔ !x. R ∧ P x ⇒ Q) ``] >>
-     FIRST_X_ASSUM (qspecl_then [`clengths`, `lex_cenv`, `next`, `cenv'''`, `inverse_cenv`, `a`, `genv_i2`, `s''`] mp_tac) >>
+     FIRST_X_ASSUM (qspecl_then [`tagenv`, `gtagenv`, `a`, `genv_i2`, `s''`] mp_tac) >>
      rw [] >>
-     fs [cenv_mapping_to_lex_cenv_def] >>
-     MAP_EVERY qexists_tac [`(c, s''''')`, `r_i2`] >>
+     fs [] >>
+     MAP_EVERY qexists_tac [`(c, s'''')`, `r_i2`] >>
      rw [] >>
      metis_tac [pat_bindings_to_i2])
  >- (pop_assum mp_tac >>
      rw [] >>
      fs [s_to_i2_cases, env_all_to_i2_cases] >>
      rw [] >>
-     `match_result_to_i2 (cenv''',clengths) No_match 
-            (pmatch_i2 s'' (pat_to_i2 lex_cenv p) v_i2 env_i2')`
+     `match_result_to_i2 gtagenv No_match 
+            (pmatch_i2 s'' (pat_to_i2 tagenv p) v_i2 env_i2')`
                    by metis_tac [pmatch_to_i2_correct, match_result_distinct] >>
-     cases_on `pmatch_i2 s'' (pat_to_i2 lex_cenv p) v_i2 env_i2'` >>
+     cases_on `pmatch_i2 s'' (pat_to_i2 tagenv p) v_i2 env_i2'` >>
      fs [match_result_to_i2_def] >>
-     rw [cenv_mapping_to_lex_cenv_def] >>
-     fs [cenv_mapping_to_lex_cenv_def,
-         METIS_PROVE [] ``(((?x. P x) ∧ R ⇒ Q) ⇔ !x. P x ∧ R ⇒ Q) ∧ ((R ∧ (?x. P x) ⇒ Q) ⇔ !x. R ∧ P x ⇒ Q) ``] >>
+     rw [] >>
+     fs [METIS_PROVE [] ``(((?x. P x) ∧ R ⇒ Q) ⇔ !x. P x ∧ R ⇒ Q) ∧ ((R ∧ (?x. P x) ⇒ Q) ⇔ !x. R ∧ P x ⇒ Q) ``] >>
      metis_tac [pat_bindings_to_i2]));
-
-val cenv_mapping_to_cenv_def = Define `
-cenv_mapping_to_cenv cenv_mapping clengths =
-   case cenv_mapping of
-     (a,b,c,d) => (c, clengths)`;
 
 val merge_envC_empty = Q.prove (
 `!envC. merge_envC (emp,emp) envC = envC ∧ merge_envC ([],[]) envC = envC`,
@@ -1043,7 +1019,25 @@ rw [emp_def] >>
 PairCases_on `envC` >>
 rw [merge_envC_def, merge_def]);
 
-(*
+     (*
+val mod_extend_empty_cenv_inv = Q.prove (
+`!envC cenv_mapping clengths.
+  cenv_inv envC cenv_mapping clengths
+  ⇒
+  cenv_inv (merge_envC (mod_cenv mn []) envC) cenv_mapping clengths`,
+ rw [mod_cenv_def] >>
+ cases_on `mn` >>
+ rw [] >>
+ PairCases_on `envC` >>
+ fs [merge_envC_def, cenv_inv_def, merge_def] >>
+ PairCases_on `cenv_mapping` >>
+ fs [cenv_inv_def] >>
+ rw [] >>
+ fs [lookup_con_id_def] >>
+ every_case_tac >>
+ fs [] >>
+ metis_tac []);
+
 val alloc_tag_cenv_inv = Q.prove (
 `!envC mn cenv types clengths x l t.
   cenv_inv envC cenv clengths ∧
@@ -1105,7 +1099,6 @@ metis_tac []
  every_case_tac >>
  fs [] >>
  rw [id_to_n_def, FLOOKUP_UPDATE]
- *)
 
 val alloc_tags_cenv_inv = Q.prove (
 `!envC mn cenv types clengths.
@@ -1116,7 +1109,6 @@ val alloc_tags_cenv_inv = Q.prove (
     cenv_weak (cenv_mapping_to_cenv cenv clengths) (cenv_mapping_to_cenv (alloc_tags mn cenv types) clengths')`,
 cheat);
 
-  (*
  induct_on `types` >>
  rw [alloc_tags_def] >>
  PairCases_on `h` >>
@@ -1126,33 +1118,88 @@ cheat);
  PairCases_on `h` >>
  rw [] >>
  res_tac
- *)
 
-val extend_cenv_inv = Q.prove (
-`!cenv_mapping ds cenv_mapping' ds_i2.
-  cenv_inv envC cenv_mapping clengths /\
-  decs_to_i2 cenv_mapping ds = (cenv_mapping', ds_i2)
+
+val gtagenv_weak_refl = Q.prove (
+`!gtagenv envC tagenv. 
+  cenv_inv envC tagenv gtagenv
+  ⇒
+  gtagenv_weak gtagenv gtagenv`,
+ rw [gtagenv_weak_def] >>
+ metis_tac [SUBMAP_REFL, cenv_inv_def]);
+
+val lookup_tag_insert_tag = Q.prove (
+`!cn cn' next tagenv.
+ lookup_tag_env (SOME cn') (insert_tag_env cn next tagenv) =
+   if Short cn = cn' then
+     next
+   else
+     lookup_tag_env (SOME cn') tagenv`,
+ rw [] >>
+ PairCases_on `tagenv` >>
+ fs [lookup_tag_env_def, insert_tag_env_def, lookup_tag_flat_def] >>
+ every_case_tac >>
+ fs [FLOOKUP_UPDATE] >>
+ cases_on `cn = a` >>
+ fs []);
+
+val alloc_tag_cenv_inv_error = Q.prove (
+`!envC tagenv_st gtagenv cn t.
+  cenv_inv envC (get_tagenv tagenv_st) gtagenv ∧
+  (!num_args t'. lookup_con_id (Short cn) envC = SOME (num_args,t') ⇒ t ≠ t')
+  ⇒
+  cenv_inv envC (get_tagenv (alloc_tag t cn tagenv_st)) gtagenv`,
+
+ rw [] >>
+ `?next tagenv inv_tagenv acc. tagenv_st = (next,tagenv,inv_tagenv,acc)` by metis_tac [pair_CASES] >>
+ fs [alloc_tag_def, get_tagenv_def] >>
+ fs [cenv_inv_def] >>
+ rw []
+
+ SIMP_TAC bool_ss [lookup_tag_insert_tag]
+ rw [lookup_tag_insert_tag] >>
+ res_tac >>
+ rw [] >>
+ fs [FLOOKUP_DEF, id_to_n_def] >>
+ metis_tac []
+
+
+ >- metis_tac []
+ >- metis_tac []
+
+
+val extend_cenv_inv_error = Q.prove (
+`!envC tagenv gtagenv ds_i2 ds tagenv_st tagenv_st'.
+  cenv_inv envC (get_tagenv tagenv_st) gtagenv /\
+  decs_to_i2 tagenv_st ds = (tagenv_st', ds_i2)
   ==>
-  ?clengths'. 
-    cenv_inv envC cenv_mapping' clengths' ∧
-    cenv_weak (cenv_mapping_to_cenv cenv_mapping clengths) (cenv_mapping_to_cenv cenv_mapping' clengths')`,
-cheat);
+  ?gtagenv'. 
+    cenv_inv envC (get_tagenv tagenv_st') gtagenv' ∧
+    gtagenv_weak gtagenv gtagenv'`,
 
-(*
  induct_on `ds` >>
  rw [decs_to_i2_def] >>
  rw [] >>
  every_case_tac >>
  fs [LET_THM]
- >- (`?cenv_mapping' ds'. decs_to_i2 cenv_mapping ds = (cenv_mapping', ds')` by metis_tac [pair_CASES] >>
+ >- metis_tac [gtagenv_weak_refl]
+ >- (`?tagenv_st' ds'. decs_to_i2 tagenv_st ds = (tagenv_st', ds')` by metis_tac [pair_CASES] >>
      fs [] >>
      metis_tac [])
- >- (`?cenv_mapping' ds'. decs_to_i2 cenv_mapping ds = (cenv_mapping', ds')` by metis_tac [pair_CASES] >>
+ >- (`?tagenv_st' ds'. decs_to_i2 tagenv_st ds = (tagenv_st', ds')` by metis_tac [pair_CASES] >>
      fs [] >>
      metis_tac [])
- >- (FIRST_X_ASSUM match_mp_tac >>
-     Q.LIST_EXISTS_TAC [`alloc_tags o' cenv_mapping l`, `ds_i2`] >>
+ >- cheat
+
+ >- (res_tac >>
+     ntac 2 (pop_assum mp_tac) >>
      rw [] >>
+     res_tac
+ 
+ FIRST_X_ASSUM match_mp_tac >>
+     Q.LIST_EXISTS_TAC [`ds_i2`, `alloc_tag (TypeExn o') s tagenv_st`] >>
+     rw [] >>
+
      pop_assum (fn _ => all_tac) >>
      pop_assum mp_tac >>
      Q.SPEC_TAC (`cenv_mapping`, `cenv_mapping`) >>
@@ -1165,12 +1212,11 @@ cheat);
 
      induct_on `h2` >>
      rw [LAMBDA_PROD, allo]
-     *)
 
 val extend_cenv_inv2 = Q.prove (
-`!cenv_mapping ds cenv_mapping' ds_i2.
+`!cenv_mapping ds cenv_mapping' ds_i2 mn.
   cenv_inv envC cenv_mapping clengths /\
-  cenv_inv (merge_envC ([],new_tds) envC) cenv_mapping' clengths' /\
+  cenv_inv (merge_envC (cenv_mod mn new_tds) envC) cenv_mapping' clengths' /\
   decs_to_i2 cenv_mapping ds = (cenv_mapping', ds_i2)
   ==>
   cenv_weak (cenv_mapping_to_cenv cenv_mapping clengths) (cenv_mapping_to_cenv cenv_mapping' clengths')`,
@@ -1192,60 +1238,64 @@ PairCases_on `cenv_mapping` >>
 rw [cenv_mapping_to_cenv_def, cenv_mapping_to_lex_cenv_def] >>
 metis_tac []);
 
+
+val get_acc_def = Define `
+get_acc (a,b,c,d) = d`;
+
 val decs_to_i2_correct = Q.prove (
 `!genv envC s1 ds r.
   evaluate_decs_i1 genv envC s1 ds r
   ⇒
-  !s1_i2 genv_i2 cenv_mapping ds_i2 cenv_mapping' genv' envC' s' res clengths.
+  !s1_i2 genv_i2 tagenv_st ds_i2 tagenv_st' genv' envC' s' res gtagenv.
     r = (s', envC', genv', res) ∧
     res ≠ SOME Rtype_error ∧
-    (cenv_mapping', ds_i2) = decs_to_i2 cenv_mapping ds ∧
-    cenv_inv envC cenv_mapping clengths ∧
-    s_to_i2' (cenv_mapping_to_cenv cenv_mapping clengths) s1 s1_i2 ∧
-    vs_to_i2 (cenv_mapping_to_cenv cenv_mapping clengths) genv genv_i2
+    (tagenv_st', ds_i2) = decs_to_i2 tagenv_st ds ∧
+    cenv_inv envC (get_tagenv tagenv_st) gtagenv ∧
+    s_to_i2' gtagenv s1 s1_i2 ∧
+    vs_to_i2 gtagenv genv genv_i2
     ⇒
-    ?genv'_i2 s'_i2 res_i2 clengths'.
+    ?genv'_i2 s'_i2 res_i2 gtagenv'.
       evaluate_decs_i2 genv_i2 s1_i2 ds_i2 (s'_i2,genv'_i2,res_i2) ∧
-      cenv_inv (merge_envC (mod_cenv mn envC') envC) cenv_mapping' clengths' ∧
-      vs_to_i2 (cenv_mapping_to_cenv cenv_mapping' clengths') genv' genv'_i2 ∧
-      s_to_i2' (cenv_mapping_to_cenv cenv_mapping' clengths') s' s'_i2 ∧
+      cenv_inv (merge_envC (emp,envC') envC) (get_tagenv tagenv_st') gtagenv' ∧
+      vs_to_i2 gtagenv' genv' genv'_i2 ∧
+      s_to_i2' gtagenv' s' s'_i2 ∧
       (res = NONE ∧ res_i2 = NONE ∨
-       ?err err_i2. res = SOME err ∧ res_i2 = SOME err_i2 ∧ result_to_i2 (\a b c. T) (cenv_mapping_to_cenv cenv_mapping' clengths') (Rerr err) (Rerr err_i2))`,
-cheat);
-(*
+       ?err err_i2. res = SOME err ∧ res_i2 = SOME err_i2 ∧ result_to_i2 (\a b c. T) gtagenv' (Rerr err) (Rerr err_i2))`,
  ho_match_mp_tac evaluate_decs_i1_ind >>
  rw [decs_to_i2_def] >>
  every_case_tac >>
  fs [LET_THM, evaluate_dec_i1_cases] >>
  rw []  
- >- (fs [emp_def, Once evaluate_decs_i2_cases, v_to_i2_eqns, s_to_i2'_cases] >>
-     PairCases_on `cenv_mapping` >>
-     fs [merge_envC_empty, cenv_inv_def, cenv_mapping_to_cenv_def] >>
-     qexists_tac `clengths` >>
-     rw [] >>
+ >- (fs [emp_def, Once evaluate_decs_i2_cases, v_to_i2_eqns, s_to_i2'_cases, merge_envC_empty] >>
      metis_tac [])
- >- (`?cenv_mapping' ds_i2. decs_to_i2 cenv_mapping ds = (cenv_mapping', ds_i2)` by metis_tac [pair_CASES] >>
+ >- (`?tagenv_st' ds_i2. decs_to_i2 tagenv_st ds = (tagenv_st', ds_i2)` by metis_tac [pair_CASES] >>
      fs [] >>
      rw [Once evaluate_decs_i2_cases] >>
      fs [s_to_i2'_cases] >>
-     `env_all_to_i2 cenv_mapping (genv,envC,emp) (genv_i2,[]) (cenv_mapping_to_cenv cenv_mapping clengths)` 
-                 by (fs [env_all_to_i2_cases, cenv_mapping_to_cenv_def] >>
+     `env_all_to_i2 (get_tagenv tagenv_st) (genv,envC,emp) (genv_i2,[]) gtagenv`
+                 by (fs [env_all_to_i2_cases] >>
                      rw [emp_def, v_to_i2_eqns] >>
                      every_case_tac >>
                      metis_tac []) >>
-     imp_res_tac exp_to_i2_correct >>
-     fs [] >>
-     pop_assum mp_tac >>
-     rw [s_to_i2_cases, s_to_i2'_cases] >>
-     res_tac >>
-     fs [] >>
-     res_tac >>
-     fs [] >>
+     `?s'_i2 r_i2 count' s'.
+        result_to_i2 v_to_i2 gtagenv (Rerr e) r_i2 ∧
+        s'_i2 = (count',s') ∧
+        vs_to_i2 gtagenv s2 s' ∧
+        evaluate_i2 F (genv_i2,[]) (0,s1_i2) (exp_to_i2 (get_tagenv tagenv_st) e') (s'_i2,r_i2)`
+           by (imp_res_tac exp_to_i2_correct >>
+               fs [] >>
+               pop_assum mp_tac >>
+               rw [s_to_i2_cases, s_to_i2'_cases] >>
+               res_tac >>
+               fs [] >>
+               res_tac >>
+               fs [] >>
+               metis_tac []) >>
      rw [evaluate_dec_i2_cases] >>
-     `?clengths'.
-       cenv_inv envC cenv_mapping' clengths' ∧
-       cenv_weak (cenv_mapping_to_cenv cenv_mapping clengths) (cenv_mapping_to_cenv cenv_mapping' clengths')` 
-                   by metis_tac [extend_cenv_inv] >>
+     `?gtagenv'.
+       cenv_inv envC (get_tagenv tagenv_st') gtagenv' ∧
+       gtagenv_weak gtagenv gtagenv'` 
+                   by metis_tac [extend_cenv_inv_error, merge_envC_empty, emp_def] >>
      fs [emp_def, result_to_i2_cases, v_to_i2_eqns] >>
      rw [merge_envC_empty] >>
      metis_tac [v_to_i2_weakening])
@@ -1312,7 +1362,6 @@ cheat);
  >- (fs [merge_envC_empty_assoc, merge_def, emp_def] >>
      FIRST_X_ASSUM match_mp_tac >>
      metis_tac [extend_cenv_inv2, v_to_i2_weakening, s_to_i2'_cases, alloc_tag_cenv_inv]));
-     *)
 
 val dummy_env_to_i2 = Q.prove (
 `!ds cenv cenv' ds'.
@@ -1340,26 +1389,28 @@ val prompt_to_i2_correct = Q.prove (
 `!genv envC s prompt r.
   evaluate_prompt_i1 genv envC s prompt r
   ⇒
-  !s1_i2 genv_i2 cenv_mapping prompt_i2 cenv_mapping' genv' envC' s' res clengths.
+  !s1_i2 genv_i2 tagenv_st prompt_i2 genv' envC' s' res gtagenv tagenv_st'.
     r = (s', envC', genv', res) ∧
     res ≠ SOME Rtype_error ∧
-    (cenv_mapping', prompt_i2) = prompt_to_i2 cenv_mapping prompt ∧
-    cenv_inv envC cenv_mapping clengths ∧
-    s_to_i2' (cenv_mapping_to_cenv cenv_mapping clengths) s s1_i2 ∧
-    vs_to_i2 (cenv_mapping_to_cenv cenv_mapping clengths) genv genv_i2
+    (tagenv_st', prompt_i2) = prompt_to_i2 tagenv_st prompt ∧
+    cenv_inv envC (FST (SND tagenv_st)) gtagenv ∧
+    s_to_i2' gtagenv s s1_i2 ∧
+    vs_to_i2 gtagenv genv genv_i2
     ⇒
-    ?genv'_i2 s'_i2 res_i2 clengths'.
+    ?genv'_i2 s'_i2 res_i2 gtagenv'.
       evaluate_prompt_i2 genv_i2 s1_i2 prompt_i2 (s'_i2,genv'_i2,res_i2) ∧
-      cenv_inv (merge_envC envC' envC) cenv_mapping' clengths' ∧
-      vs_to_i2 (cenv_mapping_to_cenv cenv_mapping' clengths') genv' genv'_i2 ∧
-      s_to_i2' (cenv_mapping_to_cenv cenv_mapping' clengths') s' s'_i2 ∧
+      cenv_inv (merge_envC envC' envC) (FST (SND tagenv_st')) gtagenv' ∧
+      vs_to_i2 gtagenv' genv' genv'_i2 ∧
+      s_to_i2' gtagenv' s' s'_i2 ∧
       (res = NONE ∧ res_i2 = NONE ∨
-       ?err err_i2. res = SOME err ∧ res_i2 = SOME err_i2 ∧ result_to_i2 (\a b c. T) (cenv_mapping_to_cenv cenv_mapping' clengths') (Rerr err) (Rerr err_i2))`,
- rw [evaluate_prompt_i1_cases, evaluate_prompt_i2_cases, prompt_to_i2_def] >>
+       ?err err_i2. res = SOME err ∧ res_i2 = SOME err_i2 ∧ result_to_i2 (\a b c. T) gtagenv' (Rerr err) (Rerr err_i2))`,
+ rw [evaluate_prompt_i1_cases, evaluate_prompt_i2_cases] >>
+ `?next tagenv inv_tagenv. tagenv_st = (next,tagenv,inv_tagenv)` by metis_tac [pair_CASES] >>
+ fs [prompt_to_i2_def] >>
  every_case_tac >>
  fs [LET_THM] >>
  rw [] >>
- `?cenv_mapping' prompt_i2. decs_to_i2 cenv_mapping ds = (cenv_mapping',prompt_i2)` by metis_tac [pair_CASES] >>
+ `?next' tagenv' inv_tagenv' acc ds_i2. decs_to_i2 (next,tagenv,inv_tagenv,[]) ds = ((next',tagenv',inv_tagenv',acc),ds_i2)` by metis_tac [pair_CASES] >>
  fs [] >>
  rw []
  >- metis_tac [decs_to_i2_correct, NOT_SOME_NONE] >>
@@ -1392,5 +1443,6 @@ val prompt_to_i2_correct = Q.prove (
                       induct_on `nn` >>
                       rw [v_to_i2_eqns, GENLIST, SNOC_APPEND, vs_to_i2_append1]) >>
      metis_tac [vs_to_i2_append]))
+     *)
 
 val _ = export_theory ();
